%\begin{enumerate}[label=(\alph*)]


Consider the constant elasticity of substitution (CES) production function

    \begin{equation}
    \begin{aligned}
    F(K,L) = (\alpha K^{\rho} + (1-\alpha)L^{\rho})^{1/\rho}
    \end{aligned}
    \end{equation}
with $\rho \in (-\infty,1]$ and $ \alpha \in (0,1)$.

\begin{itemize}
\item 
CES is CRTS

    \begin{equation}
    \begin{aligned}
    F(\lambda K,\lambda L) = (\alpha (\lambda K)^{\rho} + (1-\alpha)(\lambda L)^{\rho})^{1/\rho} \\
    F(\lambda K,\lambda L) = (\lambda^{\rho}(\alpha (K)^{\rho} + (1-\alpha)(L)^{\rho}))^{1/\rho} \\
    F(\lambda K,\lambda L) = \lambda(\alpha (K)^{\rho} + (1-\alpha)(L)^{\rho})^{1/\rho} 
    \end{aligned}
    \end{equation}

\item 
Derive conditional factor demands $(K^{c},L^{c})$ and the CES cost function.
From FOC we have ,

    \begin{equation}
    \begin{aligned}
        & F_{L} = \frac{1}{\rho}(\alpha K^{\rho} + (1-\alpha)L^{\rho})^{(1/\rho)-1}[(1-\alpha) \rho L^{\rho-1}] = w \\
        & F_{K} = \frac{1}{\rho}(\alpha K^{\rho} + (1-\alpha)L^{\rho})^{(1/\rho)-1}[\alpha \rho K^{\rho-1}] = r \\
        & \frac{F_{L}}{F_{K}} = \frac{(1-\alpha)L^{\rho-1}}{(\alpha)K^{\rho-1}}=\frac{w}{r} \\
        & K = (\frac{\alpha}{1-\alpha}\frac{w}{r})^{\frac{1}{1-\rho}}L  ;\  
        L = (\frac{r}{\alpha})^{\frac{-1}{\rho-1}}
        (\frac{w}{1-\alpha})^{\frac{1}{\rho-1}}K
    \end{aligned}
    \end{equation}

So we need to plug the last equation in the Production function for a level $F(K,L)=\bar{q}$.

    \begin{equation}
    \begin{aligned}
    F(K,L) =\bar{q} =(\alpha K^{\rho} + (1-\alpha)[(\frac{r}{\alpha})^{\frac{-1}{\rho-1}}
        (\frac{w}{1-\alpha})^{\frac{1}{\rho-1}}K]^{\rho})^{1/\rho}
    \end{aligned}
    \end{equation}

with this equation we can find the conditional demand of capital and then using the optimal condition in (7) to find the Labor demand. 

    \begin{equation}
    \begin{aligned}
    K^{c}=\frac{\bar{q}(\frac{r}{\alpha})^{\frac{1}{\rho-1}}}
        {[\alpha(\frac{r}{\alpha})^{\frac{\rho}{\rho-1}}+
        (1-\alpha)(\frac{w}{1-\alpha})^{\frac{\rho}{\rho-1}}]^{\frac{1}{\rho}}} \\
    L^{c} =\frac{\bar{q}(\frac{w}{1-\alpha})^{\frac{1}{\rho-1}}}
        {[\alpha(\frac{r}{\alpha})^{\frac{\rho}{\rho-1}}+
        (1-\alpha)(\frac{w}{1-\alpha})^{\frac{\rho}{\rho-1}}]^{\frac{1}{\rho}}} 
    \end{aligned}
    \end{equation}

then we can find the CES cost function

    \begin{equation}
    \begin{aligned}
    C(\bar{q}) = r\frac{\bar{q}(\frac{r}{\alpha})^{\frac{1}{\rho-1}}}
        {[\alpha(\frac{r}{\alpha})^{\frac{\rho}{\rho-1}}+
        (1-\alpha)(\frac{w}{1-\alpha})^{\frac{\rho}{\rho-1}}]^{\frac{1}{\rho}}} +
    w\frac{\bar{q}(\frac{w}{1-\alpha})^{\frac{1}{\rho-1}}}
        {[\alpha(\frac{r}{\alpha})^{\frac{\rho}{\rho-1}}+
        (1-\alpha)(\frac{w}{1-\alpha})^{\frac{\rho}{\rho-1}}]^{\frac{1}{\rho}}} 
    \end{aligned}
    \end{equation}

\item 
The elasticity of technical substitution for CES production.

    \begin{equation}
    \begin{aligned}
    \sigma = \frac{d\ln{K/L}}{d\ln{w/r}} =
    \frac{d\ln{(\frac{\alpha}{1-\alpha}\frac{w}{r})^{\frac{1}{1-\rho}}}}{d\ln{w/r}}=
    \frac{\frac{1}{1-\rho}
    d[{ \ln{\frac{w}{r}} + \ln{\frac{\alpha}{1-\alpha}}]
    }}{d\ln{w/r}}= \frac{1}{1-\rho}
    \end{aligned}
    \end{equation}

\item 
CES function might become into different functions depending on the values of $\rho$.
When $\rho = 1$ then we have the linear function. 

    \begin{equation}
    \begin{aligned}
    F(K,L) = \alpha K + (1-\alpha)L
    \end{aligned}
    \end{equation}

When $\rho = 0$ then we get the Cobb–Douglas production function. To prove this first we need to take ln of F(K,L) ,

    \begin{equation}
    \begin{aligned}
    \ln{F(K,L)} = \frac{1}{\rho} \ln((\alpha k^{\rho} + (1-\alpha)L^{\rho}))
    \end{aligned}
    \end{equation}

We need to use l'Hôpital's rule to show the convergence to the Cobb-Douglas function when $\lim_{\rho\to 0}\ln{F(K,L)}$ and we can use the continuity properties from the production function. 

    \begin{equation}
    \begin{aligned}
        \lim_{\rho\to 0}\ln{F(K,L)} 
        & = \lim_{\rho\to 0} \frac{\frac{1}{\alpha k^{\rho} + (1-\alpha)L^{\rho}}
        [\alpha k^{\rho}\ln{K} + (1-\alpha)L^{\rho}\ln{L}]}{1} \\
        & = \alpha \ln{K} + (1-\alpha) \ln{L} \\
        &  =  \ln(K^{\alpha}L^{(1-\alpha)}) \Longrightarrow {F(K,L)} = K^{\alpha}L^{(1-\alpha)}
    \end{aligned}
    \end{equation}

When $\lim_{\rho \to -\infty}$ then we get the $\min{(K, L)}$ production function.
This exercise is similar to do $\lim_{\rho \to \infty}F(K,L,-\rho)$ where 

    \begin{equation}
    \begin{aligned}
    F(K,L,-p) = \frac{1}{(\alpha \frac{1}{K^{\rho}} + (1-\alpha)\frac{1}{L^{\rho}})^{1/\rho}}
    \end{aligned}
    \end{equation}

Let´s propose the next function 
    \begin{equation}
    \begin{aligned}
    U(K,L) = (\alpha \frac{1}{K^{\rho}} + (1-\alpha)\frac{1}{L^{\rho}})^{1/\rho}
    \end{aligned}
    \end{equation}

If we assume that $L<K \implies \frac{\alpha}{L^{\rho}} > \frac{\alpha}{K^{\rho}}$ and  $\frac{1-\alpha}{L^{\rho}} \geq  \frac{1-\alpha}{L^{\rho}} \implies 
\frac{1}{L^{\rho}} \geq  \frac{\alpha}{K^{\rho}} + \frac{1-\alpha}{L^{\rho}}$. \\
Therefore we conclude that the upper bound of U(K,L) is 

    \begin{equation}
    \begin{aligned}
    U(K,L) = (\alpha \frac{1}{K^{\rho}} + (1-\alpha)\frac{1}{L^{\rho}})^{1/\rho} \leq\frac{1}{L} 
    \end{aligned}
    \end{equation}

But is also true that 
    \begin{equation}
    \begin{aligned}
    (1-\alpha)^{\frac{1}{\rho}}\frac{1}{L} \leq U(K,L) = (\alpha \frac{1}{K^{\rho}} + (1-\alpha)\frac{1}{L^{\rho}})^{1/\rho} \leq\frac{1}{L} 
    \end{aligned}
    \end{equation}

Since we know that $F(K,L,-p) = [U(K,L)]^{-1}$ this implies that 
    \begin{equation}
    \begin{aligned}
     L \leq 
    F(K,L,-p) = \frac{1}{(\alpha \frac{1}{K^{\rho}} + (1-\alpha)\frac{1}{L^{\rho}})^{1/\rho}} \leq
    \frac{L}{(1-\alpha)^{\frac{1}{\rho}}}
    \end{aligned}
    \end{equation}

Then when we take the  $\lim_{\rho \to \infty}\frac{L}{(1-\alpha)^{\frac{1}{\rho}}}=L$ which sandwiches the middle term in (19) to L. Therefore we have proved that $\lim_{\rho \to -\infty}F(K,L,\rho) = \min{(K, L)}$.




\end{itemize}





%\end{enumerate}